Redesign semi-automatic way to get good TCs
Previous commit was broken: termination goal for plen was probably not
provable. Here we try a different approach. Instead of inverse-eta
expanding certain monadic constants, we instead make sure that
applications of BIND and IGNORE_BIND have the right number of arguments,
and that the second argument is an abstraction with at least 2 (or 1)
bound variables.

This creates almost all the right matching conditions for TFL to operate
nicely, but there is (at least) one ugly hack required, because the
conversion can introduce terms of the form ((if b then a else c) s). The
hack is to rewrite these to (if b then a s else c s) after the
conversion, before passing off to TFL. I don't know if there may be more
cases like this that need a rewrite; probably not in any code I will
write.

hol/reduceScript.sml
@@ -3,96 +3,71 @@ open HolKernel boolLib bossLib Parse monadsyntax ptypes_definitionsTheory lcsymt
 val _ = new_theory "reduce"
 
 (*
-val STATE_OPTION_IGNORE_BIND_weak_cong = Q.store_thm(
-"STATE_OPTION_IGNORE_BIND_weak_cong",
-`(m1 = m1') ∧
- (!s''. (∃s. OPTION_MAP SND (m1' s) = SOME s'') ⇒ (m2 s'' = m2' s'')) ⇒
- (STATE_OPTION_IGNORE_BIND m1 m2 = STATE_OPTION_IGNORE_BIND m1' m2')`,
-srw_tac [boolSimps.DNF_ss][STATE_OPTION_IGNORE_BIND_def,FUN_EQ_THM] >>
-Cases_on `m1' x` >> srw_tac [][] >> PROVE_TAC []);
-val () = DefnBase.add_cong STATE_OPTION_IGNORE_BIND_weak_cong;
-(* fix drop_cong if there are going to be multiple congruences... *)
+HOW DO YOU TURN
 
-val STATE_OPTION_BIND_weak_cong = Q.store_thm(
-"STATE_OPTION_BIND_weak_cong",
-`(m = m') ∧
- (∀v s''. (∃s. (m' s = SOME (v,s''))) ⇒ (f v s'' = f' v s'')) ⇒
- (STATE_OPTION_BIND m f = STATE_OPTION_BIND m' f')`,
-srw_tac [boolSimps.DNF_ss][STATE_OPTION_BIND_def,FUN_EQ_THM] >>
-Cases_on `m' x` >> srw_tac [][pairTheory.UNCURRY] >>
-first_x_assum match_mp_tac >> srw_tac [][pairTheory.EXISTS_PROD] >>
-PROVE_TAC [] );
-val () = DefnBase.add_cong STATE_OPTION_BIND_weak_cong;
+`plen M =
+ STATE_OPTION_IGNORE_BIND
+ (λs. STATE_OPTION_LIFT (OPTION_GUARD (∃ls. list_of_List embed_Term s M ls)) s)
+ (STATE_OPTION_BIND (EmptyListOfTerms M)
+   (λb. if ¬b then
+          STATE_OPTION_BIND (TailOfListOfTerms M)
+          (λM. STATE_OPTION_BIND (plen M)
+               (λn. STATE_OPTION_UNIT (n + 1)))
+        else STATE_OPTION_UNIT 0))`
+
+INTO
+
+`plen M = \s.
+ STATE_OPTION_IGNORE_BIND
+ (λs. STATE_OPTION_LIFT (OPTION_GUARD (∃ls. list_of_List embed_Term s M ls)) s)
+ (\s. STATE_OPTION_BIND (EmptyListOfTerms M)
+      (λb.\s. if ¬ b
+             then STATE_OPTION_BIND (TailOfListOfTerms M)
+                  (λM. \s. STATE_OPTION_BIND (plen M)
+                         (λn.\s. STATE_OPTION_UNIT (n+1) s)
+                         s)
+                  s
+             else (STATE_OPTION_UNIT 0 s))
+      s)
+ s`
+
+GENERICALLY?
+
+is COND the only special case?
+i.e. use this
+`if b then c else a = (λx. if b then c x else a x)
+instead of ETA_AX whenever it applies
+
+or alternatively, run a simplification phase with
+`(if b then c else a) x = if b then c x else a x`
+after doing normal uneta
 *)
 
 (*
-val tm = ``foo a1 a2``
-val (rator,rand) = dest_comb tm
-val th = SIMP_CONV pure_ss [Ntimes (GSYM BETA_THM) 2] ``bar a1 a2 a3``;
+(* Examples of desired definitions *)
+val foo_defn = Hol_defn "foo"
+`foo M = do
+  b <- return F ;
+  if b then foo M else return () ;
+  return ()
+od`;
 
-val INVERSE_ETA_THM = save_thm(
-"INVERSE_ETA_THM",
-FUN_EQ_THM |>  Q.SPEC `f` |> Q.SPEC `\x. f x` |> EQ_IMP_RULE |> snd
-|> UNDISCH |> PROVE_HYP (BETA_THM |> GSYM |> Q.SPEC `f`)
-|> Q.GEN `f`);
+val ignore_rec_defn = Hol_defn "ignore_rec"
+`ignore_rec = STATE_OPTION_IGNORE_BIND
+              (λs. OPTION_MAP (combin$C $, s) (OPTION_GUARD (s T)))
+              (λs. ignore_rec ((T =+ ¬(s T)) s))`;
 
-val th1 = 
-((RATOR_CONV (SIMP_CONV pure_ss [Once INVERSE_ETA_THM])) THENC
-(fn tm => RATOR_CONV (ALPHA_CONV (snd(dest_comb tm))) tm))
-``bar a1``
-
-val th2 =
-((RATOR_CONV (SIMP_CONV pure_ss [Once INVERSE_ETA_THM])) THENC
-(fn tm => RATOR_CONV (ALPHA_CONV (snd(dest_comb tm))) tm))
-``bar a1 a2``
-
-SIMP_CONV pure_ss [Once th1] ``bar a1 a2``
-INVERSE_ETA_THM
-th2
-SUBS [th1] th2
-SUBS_OCCS [([2],th1)] th2
-GSYM (SUBST_MATCH th1 (GSYM th2))
-
-ONCE_REWRITE_RULE [th1] th2
-help"SUBS_OCCS";
-
-CONV_RULE BETA_CONV it
-help"SimpRHS"
-
-CONV_RULE (RAND_CONV (ONCE_DEPTH_CONV ETA_CONV)) th
-ETA_CONV
-ETA_RULE
-ETA
+val plen_defn = Hol_defn "plen"
+`plen M = do
+  (λs. STATE_OPTION_LIFT (OPTION_GUARD (∃ls. list_of_List embed_Term s M ls)) s) ;
+  b <- EmptyListOfTerms M ;
+  if ¬b then do
+    M <- TailOfListOfTerms M ;
+    n <- plen M ;
+    return (n + 1)
+  od else return 0
+od`;
 *)
-
-(*
-val () = use "/home/ramana/HOL/src/tfl/src/RW.sml";
-val () = use "/home/ramana/HOL/src/tfl/src/Defn.sml";
-val () = RW.monitoring := true;
-*)
-
-(*
-fun GNOT_ABS_INVERSE_ETA_CONV t = let
-  val _ = assert (not o pairLib.is_pabs) t
-in
-  INVERSE_ETA_CONV (genvar(#1(dom_rng(type_of t)))) t
-end handle e => raise wrap_exn "" "GNOT_ABS_INVERSE_ETA_CONV" e
-
-fun VNOT_ABS_INVERSE_ETA_CONV s t = let
-  val _ = assert (not o pairLib.is_pabs) t
-  val vs = free_vars t
-in
-  INVERSE_ETA_CONV (prim_variant vs (mk_var (s,(#1(dom_rng(type_of t)))))) t
-end handle e => raise wrap_exn "" "VNOT_ABS_INVERSE_ETA_CONV" e
-
-fun VCOMB_INVERSE_ETA_CONV s t = let
-  val _ = assert is_comb t
-  val vs = free_vars t
-in
-  INVERSE_ETA_CONV (prim_variant vs (mk_var (s,(#1(dom_rng(type_of t)))))) t
-end handle e => raise wrap_exn "" "VCOMB_INVERSE_ETA_CONV" e
-*)
-
 
 (* Conversions for selectively applying (inverse) eta on certain constants *)
 
@@ -106,6 +81,7 @@ fun UNETA_CONV x t =
   end
   handle e => raise wrap_exn "" "UNETA_CONV" e
 
+(*
 fun UNETA_THESE_CONV ts x t = let
   val (rator,_) = strip_comb t
   val _ = assert (exists (can (C match_term rator))) ts
@@ -119,6 +95,7 @@ fun ETA_THESE_CONV ts t = let
 in
   ETA_CONV t
 end handle e => raise wrap_exn "" "ETA_THESE_CONV" e
+*)
 
 local
   (* Insert all definitions required to get Defn.parse_from_absyn here.
@@ -248,7 +225,7 @@ local
    in
      (Absyn.list_mk_conj (rev eql), rev fset)
    end
-
+in
   fun parse_absyn absyn0 =
    let val (absyn,fn_names) = elim_wildcards absyn0
        val restore_these = map (fn s => (s, Parse.hide s)) fn_names
@@ -261,17 +238,18 @@ local
      restore();
      (tm, fn_names)
    end
-in
-  fun qrule ts x q = let
-    val (t,_) = parse_absyn (Parse.Absyn q)
-    fun term_to_quote t = [QUOTE (term_to_string t) : term frag]
-    val th = DEPTH_CONV (UNETA_THESE_CONV ts x) t handle UNCHANGED => REFL t
-    val t = rhs (concl th)
-  in
-    term_to_quote t
-  end
-  fun unconv_rule ts = CONV_RULE (DEPTH_CONV (ETA_THESE_CONV ts))
 end
+
+(*
+fun qrule ts x q = let
+  val (t,_) = parse_absyn (Parse.Absyn q)
+  fun term_to_quote t = [QUOTE (term_to_string t) : term frag]
+  val th = DEPTH_CONV (UNETA_THESE_CONV ts x) t handle UNCHANGED => REFL t
+  val t = rhs (concl th)
+in
+  term_to_quote t
+end
+fun unconv_rule ts = CONV_RULE (DEPTH_CONV (ETA_THESE_CONV ts))
 
 val state_option_consts =
 [``STATE_OPTION_BIND``,
@@ -309,21 +287,277 @@ srw_tac [][combinTheory.APPLY_UPDATE_THM,OPTION_GUARD_def]);
 val (ignore_rec_def,ignore_rec_ind) =
 W (curry op ##) (unconv_rule state_option_consts) p;
 
-val plen_defn = Defn.Hol_defn "plen" (
-qrule state_option_consts ``s:state`` `
+task: write a conversion that recursively makes sure any occurrence of
+STATE_OPTION_BIND is of the form STATE_OPTION_BIND m (\v s. f) s, and any occurrence of
+STATE_OPTION_IGNORE_BIND is of the form STATE_OPTION_IGNORE_BIND m1 (\s. m2) s
+
+possible algorithm (do DEPTH_CONV on this):
+if you encounter an application of (unit)bind in the wrong form:
+if it has only 2 arguments, inverse eta yourself.
+if the second argument doesn't have enough bound variables, inverse eta as appropriate.
+
+better algorithm (incorporated DEPTH_CONV):
+entry point with no current argument:
+  perform inverse eta then recurse on rator with introduce variable as current argument
+entry point with a current argument s:
+  if tm = BIND m f then
+    m' <- recurse on m with no current argument
+    ensure f is of the form (\v s'. g) by inverse eta if necessary
+    g' <- recurse on g with current argument s'
+    return BIND m (\v s'. g') s
+  else if tm = IGNORE_BIND m1 m2 then
+    m1' <- recurse on m with no current argument
+    ensure m2 is of the form (\s'. g) by inverse eta if necessary
+    g' <- recurse on g with current argument s'
+    return IGNORE_BIND m1' (\s'. g') s
+  else if tm = (λx. f) then return f s
+  else if tm = x then return x s
+  else if tm = con then return con s
+  else if tm = (rator rand) then
+    ??????
+
+keep track of the current state argument
+if initially there is no state argument, do an inverse eta to get one, then recurse on rator and current argument
+if rator is a BIND form, do something special:
+  BIND m f s - recurse on m with no current argument
+               make sure f is of the form (\v s. g) by inverse eta if necessary
+               recurse on g with current argument s
+otherwise, remove the argument and push it into the recursion on the rator instead
+
+
+test on this:
+`plen M = do
+  (λs. STATE_OPTION_LIFT (OPTION_GUARD (∃ls. list_of_List embed_Term s M ls)) s) ;
+  b <- EmptyListOfTerms M ;
+  if ¬b then do
+    M <- TailOfListOfTerms M ;
+    n <- plen M ;
+    return (n + 1)
+  od else return 0
+od`
+
+aka:
+`plen M =
+ STATE_OPTION_IGNORE_BIND
+ (λs. STATE_OPTION_LIFT (OPTION_GUARD (∃ls. list_of_List embed_Term s M ls)) s)
+ (STATE_OPTION_BIND (EmptyListOfTerms M)
+   (λb. if ¬b then
+          STATE_OPTION_BIND (TailOfListOfTerms M)
+          (λM. STATE_OPTION_BIND (plen M)
+               (λn. STATE_OPTION_UNIT (n + 1)))
+        else STATE_OPTION_UNIT 0))`
+
+algorithm should give:
+`plen M =
+\s. STATE_OPTION_IGNORE_BIND
+ (λs. STATE_OPTION_LIFT (OPTION_GUARD (∃ls. list_of_List embed_Term s M ls)) s)
+ (\s.
+  STATE_OPTION_BIND (EmptyListOfTerms M)
+   (λb. \s.
+        (if ¬b then
+           \s.
+           STATE_OPTION_BIND (TailOfListOfTerms M)
+           (λM. \s.
+                STATE_OPTION_BIND (plen M)
+                (λn. \s. STATE_OPTION_UNIT (n + 1) s)
+                s)
+           s
+         else STATE_OPTION_UNIT 0)
+        s)
+  s)
+s`
+but this isn't good enough!
+need to BETA_RULE through the if !
+*)
+
+(*
+fun strip_type ty = let
+  val (dom,rng) = dom_rng ty
+in dom::(strip_type rng)
+end handle HOL_ERR _ => [ty]
+
+val arity = let
+  fun loop n ty = let
+    val (dom,rng) = dom_rng ty
+  in loop (n+1) rng end
+  handle HOL_ERR _ => n
+in loop 0 end
+*)
+
+(* make sure tm is an abstraction of at least (length vs) variables, using
+variables from vs (in reverse order) for inverse eta-expansion if necessary.
+if an element of vs is NONE, use a genvar instead *)
+
+local
+  fun GEN_UNETA_CONV NONE tm = let
+    val (dom,_) = dom_rng (type_of tm)
+  in UNETA_CONV (genvar dom) tm end
+    | GEN_UNETA_CONV (SOME x) tm = UNETA_CONV x tm
+in
+  fun VLIST_CONV vs tm = let
+    val (ws,m) = strip_abs tm
+    val vs = List.drop(vs,length ws)
+  in
+    STRIP_BINDER_CONV NONE (EVERY_CONV (map GEN_UNETA_CONV vs)) tm
+  end
+end
+
+local
+  val unitbind = ``STATE_OPTION_IGNORE_BIND :
+    ('a,'b) state_option -> ('a,'c) state_option -> ('a,'c) state_option``
+  val bind = ``STATE_OPTION_BIND :
+    ('a,'b) state_option -> ('b -> ('a,'c) state_option) -> ('a,'c) state_option``
+  fun f (ls,bind) s (rator,(_::_::rest)) = let
+    val (_,t) = match_term bind rator
+    val ty = valOf (subst_assoc (equal alpha) t) handle Option => alpha
+    val conv = RAND_CONV (VLIST_CONV (ls@[SOME s]))
+  in
+    case rest of
+      [] => conv THENC (UNETA_CONV s)
+    | _  => conv
+  end
+in
+  fun state_option_conv s tm = let
+    val p as (rator,_) = strip_comb tm
+    val _ = assert is_const rator
+  in
+    trye (f ([],unitbind) s) p handle HOL_ERR _ =>
+    with_exn (f ([NONE],bind) s) p
+    (mk_HOL_ERR "" "state_option_conv" "Not an application of a state_option bind")
+  end tm
+  fun state_option_unconv ty tm = let
+    val (v,m) = dest_abs tm
+  in if type_of v = ty then ETA_CONV tm else let
+    val (v,m) = dest_abs m
+  in if type_of v = ty then ABS_CONV ETA_CONV tm else
+    raise mk_HOL_ERR "" "state_option_unconv" "Not a state_option abstraction"
+  end end
+end
+
+val APPLY_COND_THM = Q.store_thm(
+"APPLY_COND_THM",
+`(if b then c else a) x = if b then c x else a x`,
+srw_tac [][]);
+
+fun qrule x q = let
+  val (t,_) = parse_absyn (Parse.Absyn q)
+  fun term_to_quote t = [QUOTE (term_to_string t) : term frag]
+  val conv = DEPTH_CONV (state_option_conv x) THENC
+             PURE_REWRITE_CONV [APPLY_COND_THM]
+  val th = conv t handle UNCHANGED => REFL t
+  val t = rhs (concl th)
+in
+  term_to_quote t
+end
+
+fun unconv_rule x = CONV_RULE (DEPTH_CONV (state_option_unconv x))
+
+(* state_option_conv ``s:state`` ``STATE_OPTION_BIND (EmptyListOfTerms M) (λb. STATE_OPTION_UNIT ())`` *)
+
+(*
+(DEPTH_CONV (state_option_conv ``s:state``) o Term)
+`plen M =
+ STATE_OPTION_IGNORE_BIND
+ (λs. STATE_OPTION_LIFT (OPTION_GUARD (∃ls. list_of_List embed_Term s M ls)) s)
+ (STATE_OPTION_BIND (EmptyListOfTerms M)
+   (λb. if ¬b then
+          STATE_OPTION_BIND (TailOfListOfTerms M)
+          (λM. STATE_OPTION_BIND (plen M)
+               (λn. STATE_OPTION_UNIT (n + 1)))
+        else STATE_OPTION_UNIT 0))`
+*)
+
+val foo_defn = Defn.Hol_defn "foo" (
+qrule ``s:'a`` `
+foo M =
+  STATE_OPTION_BIND (STATE_OPTION_UNIT F)
+  (λb. STATE_OPTION_IGNORE_BIND
+         (if b then foo M else STATE_OPTION_UNIT ())
+         (STATE_OPTION_UNIT ()))`);
+(* prove the termination goal *)
+val p = Defn.tprove (foo_defn,
+WF_REL_TAC `REMPTY` >>
+srw_tac [][STATE_OPTION_UNIT_def]);
+(* extract the theorems the user wants to see *)
+val (foo_def,foo_ind) = W (curry op ##) (unconv_rule ``:'a``) p;
+
+(* Same procedure works for this example.
+A separate bug is that you can't remove the s argument from both sides of this
+quote. *)
+val ignore_rec_defn = Defn.Hol_defn "ignore_rec" (
+qrule ``s:'a`` `
+  ignore_rec s = STATE_OPTION_IGNORE_BIND
+                 (λs. OPTION_MAP (combin$C $, s) (OPTION_GUARD (s T)))
+                 (λs. ignore_rec ((T =+ ¬(s T)) s))
+                 s`);
+val p = Defn.tprove (ignore_rec_defn,
+WF_REL_TAC `measure (λs. if s T then 1 else 0)` >>
+srw_tac [][combinTheory.APPLY_UPDATE_THM,OPTION_GUARD_def]);
+val (ignore_rec_def,ignore_rec_ind) =
+W (curry op ##) (unconv_rule alpha) p;
+
+(*
+Ideally, TFL would automatically try inverse eta to match congruences itself!
+
+(DEPTH_CONV (state_option_conv ``s:state``) o Term ) `
   plen M = do
     (λs. STATE_OPTION_LIFT (OPTION_GUARD (∃ls. list_of_List embed_Term s M ls)) s) ;
     b <- EmptyListOfTerms M ;
-    n <- if ¬ b then do
+    if ¬ b then do
       M <- TailOfListOfTerms M ;
-      plen M
-    od else return 0 ;
-    return (n + 1)
+      n <- plen M ;
+      return (n + 1)
+    od else return 0
+  od`
+
+val plen_defn = Defn.Hol_defn "plen"
+`plen M = \s.
+ STATE_OPTION_IGNORE_BIND
+ (λs. STATE_OPTION_LIFT (OPTION_GUARD (∃ls. list_of_List embed_Term s M ls))
+      s)
+ (λs. STATE_OPTION_BIND
+      (EmptyListOfTerms M)
+      (λb s. if ¬ b
+             then STATE_OPTION_BIND
+                  (TailOfListOfTerms M)
+                  (λM s. STATE_OPTION_BIND
+                         (plen M)
+                         (λn s. STATE_OPTION_UNIT (n+1) s)
+                         s)
+                  s
+             else (STATE_OPTION_UNIT 0 s))
+      s)
+ s`
+*)
+
+val plen_defn = Defn.Hol_defn "plen" (
+qrule ``s:state`` `
+  plen M = do
+    (λs. STATE_OPTION_LIFT (OPTION_GUARD (∃ls. list_of_List embed_Term s M ls)) s) ;
+    b <- EmptyListOfTerms M ;
+    if ¬ b then do
+      M <- TailOfListOfTerms M ;
+      n <- plen M ;
+      return (n + 1)
+    od else return 0
   od`)
 val p = Defn.tprove (plen_defn,
-(* I haven't proved termination here yet, because it's a lot more difficult
-here, but I am semi-confident that the termination goal is (at last) provable
-*)
+srw_tac [boolSimps.DNF_ss][pairTheory.FORALL_PROD] >>
+srw_tac [][STATE_OPTION_LIFT_def,OPTION_GUARD_def] >>
+WF_REL_TAC `measure (λM. LEAST n. ∃s ls. list_of_List embed_Term s M ls ∧ (n = LENGTH ls))` >>
+srw_tac [][] >>
+numLib.LEAST_ELIM_TAC >>
+srw_tac [][] >- metis_tac [] >>
+fsrw_tac [boolSimps.DNF_ss][] >>
+`¬ (LENGTH ls < LENGTH ls')` by METIS_TAC [] >>
+numLib.LEAST_ELIM_TAC >>
+srw_tac [][] >- (
+  fsrw_tac [][TailOfList_def,STATE_OPTION_BIND_def,pairTheory.UNCURRY] >>
+  Cases_on `M` >> fsrw_tac [][raw_lookup_def,STATE_OPTION_IGNORE_BIND_def] >>
+  fsrw_tac [][STATE_OPTION_UNIT_def] >>
+  METIS_TAC [] ) >>
+would want some TailOfList correctness results here to make things easier...
+
 )
 val (plen_def,plen_ind) =
 W (curry op ##) (unconv_rule state_option_consts) p;
@@ -331,6 +565,21 @@ W (curry op ##) (unconv_rule state_option_consts) p;
 (* You can then use save_thm to save the right form of the definition and
 induction. There are no extra flags or tags necessary to completely emulate
 Define, right? *)
+
+SIMP_CONV (srw_ss()) [] (Term  `ifcong n = (if n = 0 then EVERY ifcong else NULL) [1]`);
+DefnBase.read_congs()
+
+val ifcong_defn = Defn.Hol_defn "ifcong"
+  `ifcong n = (if n = 0 then EVERY ifcong else NULL) [1]`;
+
+val ifcong2_defn = Defn.Hol_defn "ifcong2"
+  `ifcong2 n = (if n = 0 then (λls. EVERY ifcong2 ls) else NULL) [1]`;
+
+val ifcong3_defn = Defn.Hol_defn "ifcong3"
+  `ifcong3 n = (if n = 0 then (λls. (ls = [1]) ∧ EVERY ifcong3 ls) else NULL) [1]`;
+
+foo 0 = EVERY foo [1] = foo 1 = NULL [1] = F
+foo 1 = NULL [1] = F
 
 (*
 val fail = Hol_defn "ignore_rec" Term`
